Switch to Iterator for ProofData

correctness/RegexCorrectness/NFA/Semantics/ProofData/Loop.lean
@@ -1,9 +1,9 @@
 import RegexCorrectness.NFA.Semantics.ProofData.Basic
 import RegexCorrectness.NFA.Semantics.ProofData.Compile
 
-open Regex.Data (Span)
-
 set_option autoImplicit false
+
+open String (Iterator)
 
 namespace Regex.NFA.Compile.ProofData.Star
 
@@ -16,28 +16,28 @@ it must have looped `nfaExpr` before `n` times, followed by the last step from `
 A `Loop` term corresponds to such a loop. The `last` variant corresponds to the last step,
 and the `loop` variant extracts the first iteration and the remaining loop.
 -/
-inductive Loop : Span → Span → List (Nat × String.Pos) → Prop where
-  | last {span} (step : nfa'.Step nfa.nodes.size nfa'.start span next span .none) : Loop span span []
-  | loop {span span' span'' update₁ update₂}
-    (path : nfa'.Path nfaPlaceholder.nodes.size nfaExpr.start span nfaPlaceholder.start span' update₁)
-    (loop : Loop span' span'' update₂) : Loop span span'' (update₁ ++ update₂)
+inductive Loop : Iterator → Iterator → List (Nat × String.Pos) → Prop where
+  | last {it} (step : nfa'.Step nfa.nodes.size nfa'.start it next it .none) : Loop it it []
+  | loop {it it' it'' update₁ update₂}
+    (path : nfa'.Path nfaPlaceholder.nodes.size nfaExpr.start it nfaPlaceholder.start it' update₁)
+    (loop : Loop it' it'' update₂) : Loop it it'' (update₁ ++ update₂)
 
-theorem Loop.introAux {i span j span' update}
+theorem Loop.introAux {i it j it' update}
   (lt : i < nfa'.nodes.size) (wf : nfa.WellFormed) (next_lt : next < nfa.nodes.size) (eqj : j = next)
-  (path : nfa'.Path nfa.nodes.size i span j span' update) :
+  (path : nfa'.Path nfa.nodes.size i it j it' update) :
   if i = nfa'.start then
-    (nfa'.Step nfa.nodes.size nfa'.start span next span' .none ∧ span' = span ∧ update = []) ∨
-    (∃ spanm update₁ update₂,
-      nfa'.Path nfaPlaceholder.nodes.size nfaExpr.start span nfaPlaceholder.start spanm update₁ ∧
-      Loop spanm span' update₂ ∧
+    (nfa'.Step nfa.nodes.size nfa'.start it next it' .none ∧ it' = it ∧ update = []) ∨
+    (∃ itm update₁ update₂,
+      nfa'.Path nfaPlaceholder.nodes.size nfaExpr.start it nfaPlaceholder.start itm update₁ ∧
+      Loop itm it' update₂ ∧
       update = update₁ ++ update₂)
   else
-    ∃ spanm update₁ update₂,
-      nfa'.Path nfaPlaceholder.nodes.size i span nfaPlaceholder.start spanm update₁ ∧
-      Loop spanm span' update₂ ∧
+    ∃ itm update₁ update₂,
+      nfa'.Path nfaPlaceholder.nodes.size i it nfaPlaceholder.start itm update₁ ∧
+      Loop itm it' update₂ ∧
       update = update₁ ++ update₂ := by
   induction path with
-  | @last i span j span' update step =>
+  | @last i it j it' update step =>
     split
     next eqi =>
       subst eqi eqj
@@ -48,23 +48,23 @@ theorem Loop.introAux {i span j span' update}
       have : nfa'[nfa'.start]'wf'.start_lt = .split nfaExpr.start next := by
         simp [start_eq, get_start]
 
-      exact .inl (.splitRight (Nat.le_of_eq start_eq.symm) wf'.start_lt this)
+      exact .inl (.splitRight (Nat.le_of_eq start_eq.symm) wf'.start_lt this step.2.2)
     next nei =>
       have : nfa.nodes.size ≤ i := step.ge
       have : i ≠ nfa.nodes.size := start_eq ▸ nei
       have gt : i > nfa.nodes.size := by omega
 
-      have step : nfa'.Step (nfa.nodes.size + 1) i span j span' update :=
+      have step : nfa'.Step (nfa.nodes.size + 1) i it j it' update :=
         step.liftBound' gt
-      have step : nfa'.Step nfaPlaceholder.nodes.size i span j span' update := by
+      have step : nfa'.Step nfaPlaceholder.nodes.size i it j it' update := by
         simp [nfaPlaceholder, step]
-      have step : nfaExpr.Step nfaPlaceholder.nodes.size i span j span' update :=
+      have step : nfaExpr.Step nfaPlaceholder.nodes.size i it j it' update :=
         step.cast (get_ne_start i step.lt (Nat.ne_of_gt gt))
 
       have := step.eq_or_ge_of_pushRegex
       simp [nfaPlaceholder, eqj] at this
       omega
-  | @more i span j span' k span'' update₁ update₂ step rest ih =>
+  | @more i it j it' k it'' update₁ update₂ step rest ih =>
     have ih' := ih rest.lt eqj
     split
     next eqi =>
@@ -90,40 +90,40 @@ theorem Loop.introAux {i span j span' update}
       split at ih'
       next eqj =>
         match ih' with
-        | .inl ⟨step', hspan, hupdate⟩ =>
-          simp [hspan, hupdate, eqj] at *
-          refine ⟨span', List.ofOption update₁, ?_, [], .last step', by simp⟩
+        | .inl ⟨step', hit, hupdate⟩ =>
+          simp [hit, hupdate, eqj] at *
+          refine ⟨it', List.ofOption update₁, ?_, [], .last step', by simp⟩
           simp [nfaPlaceholder]
 
           have path := Path.last (step.liftBound' gt)
           exact start_eq ▸ path
-        | .inr ⟨spanm, update₃, update₄, path', loop', equ⟩ =>
+        | .inr ⟨itm, update₃, update₄, path', loop', equ⟩ =>
           have loop'' := Loop.loop path' loop'
-          refine ⟨span', List.ofOption update₁, update₃ ++ update₄, ?_, loop'', by simp [equ]⟩
+          refine ⟨it', List.ofOption update₁, update₃ ++ update₄, ?_, loop'', by simp [equ]⟩
           simp [nfaPlaceholder]
 
-          have step : nfa'.Step nfa.nodes.size i span nfa.nodes.size span' update₁ :=
+          have step : nfa'.Step nfa.nodes.size i it nfa.nodes.size it' update₁ :=
             have : j = nfa.nodes.size := eqj ▸ start_eq
             this ▸ step
           exact (.last (step.liftBound' gt))
       next nej =>
-        have ⟨spanm, update₃, update₄, path', loop', equ⟩ := ih'
-        have step : nfa'.Step nfaPlaceholder.nodes.size i span j span' update₁ := by
+        have ⟨itm, update₃, update₄, path', loop', equ⟩ := ih'
+        have step : nfa'.Step nfaPlaceholder.nodes.size i it j it' update₁ := by
           simp [nfaPlaceholder]
           exact step.liftBound' gt
-        exact ⟨spanm, update₁ ::ₒ update₃, update₄, .more step path', loop', by simp [equ]⟩
+        exact ⟨itm, update₁ ::ₒ update₃, update₄, .more step path', loop', by simp [equ]⟩
 
-theorem Loop.intro {span span' update}
+theorem Loop.intro {it it' update}
   (wf : nfa.WellFormed) (next_lt : next < nfa.nodes.size)
-  (path : nfa'.Path nfa.nodes.size nfa'.start span next span' update) :
-  Loop span span' update := by
+  (path : nfa'.Path nfa.nodes.size nfa'.start it next it' update) :
+  Loop it it' update := by
   have wf' := wf' wf next_lt
   have loop := introAux wf'.start_lt wf next_lt rfl path
   simp at loop
   match loop with
-  | .inl ⟨step, hspan, hupdate⟩ =>
-    simp [hspan, hupdate] at *
+  | .inl ⟨step, hit, hupdate⟩ =>
+    simp [hit, hupdate] at *
     exact .last step
-  | .inr ⟨span'', update₁, path, update₂, loop, equ⟩ => exact equ ▸ Loop.loop path loop
+  | .inr ⟨it'', update₁, path, update₂, loop, equ⟩ => exact equ ▸ Loop.loop path loop
 
 end Regex.NFA.Compile.ProofData.Star
